Update ty_list of RustHalt

nola/examples/rust_halt/verify/list.v
@@ -1,6 +1,6 @@
 (** * Singly linked list type *)
 
-From nola.examples.rust_halt Require Export rec mod sum box prod.
+From nola.examples.rust_halt Require Export rec mod sum prod box.
 
 Section list.
   Context `{!rust_haltGS CON Σ, !rust_haltC CON, !rust_haltJ CON JUDG Σ,
@@ -27,7 +27,7 @@ Section list.
   (** [ty_list_gen]: Generator of the list type *)
   Definition ty_list_gen' {X} (T : ty CON Σ X) (Self : ty CON Σ (listₓ X))
     : ty CON Σ (unitₓ +ₓ X *'ₓ listₓ X) :=
-    ty_sum ty_unit (ty_box (ty_prod T Self)).
+    ty_sum ty_unit (ty_prod T (ty_box Self)).
   Definition ty_list_gen {X} (T : ty CON Σ X) (Self : ty CON Σ (listₓ X))
     : ty CON Σ (listₓ X) :=
     ty_mod (X:=unitₓ +ₓ X *'ₓ listₓ X) (Y:=listₓ X)
@@ -37,7 +37,7 @@ Section list.
     Productive (@ty_list_gen X T).
   Proof.
     move=> k ???. apply: ty_mod_preserv. apply: ty_sum_preserv=>//.
-    apply ty_box_productive. destruct k=>//=. exact: ty_prod_preserv.
+    apply ty_prod_preserv=>//. exact: ty_box_productive.
   Qed.
 
   (** [ty_list]: List type *)
@@ -45,16 +45,16 @@ Section list.
     ty_rec (ty_list_gen T).
 
   (** [ty_list] satisfies [Ty] *)
-  #[export] Instance ty_list_ty {X T} : Ty (ty_list (X:=X) T).
+  #[export] Instance ty_list_ty `{!Ty (X:=X) T} : Ty (ty_list (X:=X) T).
   Proof. exact _. Qed.
 
   (** [ty_list] satisfies [TyOp] *)
-  #[export] Instance ty_list_ty_op `(!Ty (X:=X) T, !TyOpLe T κ 1 d) :
+  #[export] Instance ty_list_ty_op `(!Ty (X:=X) T, !TyOpLe T κ 0 d) :
     TyOpAt (ty_list T) κ d.
   Proof.
-    apply (ty_rec_ty_op (F:=ty_list_gen T) ᵖ[(T, 1)'])=>/=; [|exact _]=> ??[??].
-    apply: ty_mod_ty_op. apply: ty_sum_ty_op. apply: ty_box_ty_op=> ??.
-    apply: ty_prod_ty_op; by apply ty_op_le.
+    apply (ty_rec_ty_op (F:=ty_list_gen T) ᵖ[(T, 0)'])=>/=; [|exact _]=> ??[??].
+    apply: ty_mod_ty_op. apply: ty_sum_ty_op. apply: ty_prod_ty_op.
+    exact: ty_op_le.
   Qed.
 
   (** [ty_list] preserves [Send] *)
@@ -65,27 +65,27 @@ Section list.
   Proof. exact _. Qed.
 
   (** [Resol] over [ty_list] *)
-  #[export] Instance resol_list `(!ResolLe (X:=X) T κ post 1 d) :
+  #[export] Instance resol_list `(!ResolLe (X:=X) T κ post 0 d) :
     ResolAt (ty_list T) κ (λ xl, Forall post xl) d.
   Proof.
-    apply (ty_rec_resol (F:=ty_list_gen T) ᵖ[(T, post, 1)'])=>/=; [|exact _].
+    apply (ty_rec_resol (F:=ty_list_gen T) ᵖ[(T, post, 0)'])=>/=; [|exact _].
     move=> ??[??]. eapply resol_post.
-    { apply @resol_mod, @resol_sum; [exact: _|]. eapply resol_box=> ??.
-      eapply resol_post; [apply @resol_prod; exact: resol_le'|done]. }
+    { apply @resol_mod, @resol_sum; [exact: _|].
+      apply @resol_prod; [exact: resol_le'|exact: resol_box]. }
     move=>/= [|??]//= ?. by apply Forall_cons.
   Qed.
 
   (** [Real] over [ty_list] *)
-  #[export] Instance real_list `(!RealLe (X:=X) (A:=A) T κ get 1 d) :
+  #[export] Instance real_list `(!RealLe (X:=X) (A:=A) T κ get 0 d) :
     RealAt (ty_list T) κ (λ xl, get <$> xl) d.
   Proof.
-    apply (ty_rec_real (F:=ty_list_gen T) ᵖ[(T, existT A get, 1)'])=>/=;
+    apply (ty_rec_real (F:=ty_list_gen T) ᵖ[(T, existT A get, 0)'])=>/=;
       [|exact _]=> ??[??].
     eapply real_eq.
     { apply @real_mod. eapply (real_compose list_wrap).
-      apply @real_sum; [exact: _|]. apply real_box=> ??.
-      eapply real_eq; [apply @real_prod; exact: real_le|done]. }
-    move=> [|??]//=.
+      apply @real_sum; [exact: _|].
+      apply @real_prod; [exact: real_le|exact: real_box]. }
+    move=>/= [|??]//=.
   Qed.
   #[export] Instance real_list_length {X T κ} :
     Real (ty_list (X:=X) T) κ (λ xl, length xl).
@@ -98,15 +98,15 @@ Section list.
   Lemma ty_list_unfold {X T} :
     ty_list (X:=X) T ≡ ty_list_gen T (ty_list (X:=X) T).
   Proof. exact ty_rec_unfold. Qed.
-  Lemma subty_list_fold {X T δ} :
+  Lemma subty_list_fold `{!Ty (X:=X) T} {δ} :
     ⊢ subty δ (ty_list_gen' T (ty_list T)) (ty_list (X:=X) T) list_wrap.
   Proof.
     erewrite subty_proper_fun.
     { iApply subty_trans; [|by iApply subty_rec_fold].
-      iApply (subty_to_mod (T:=ty_list_gen' _ _))=> ?. exact list_unwrap_wrap. }
-    move=>/= [[]|[??]]//=.
+      iApply (subty_to_mod (T:=ty_list_gen' T _))=> ?. exact list_unwrap_wrap. }
+    move=>/= [[]|?]//=.
   Qed.
-  Lemma subty_list_unfold {X T δ} :
+  Lemma subty_list_unfold `{!Ty (X:=X) T} {δ} :
     ⊢ subty δ (ty_list (X:=X) T) (ty_list_gen' T (ty_list T)) list_unwrap.
   Proof.
     erewrite subty_proper_fun.
